more

Weidenbach_Book/IsaSAT_Decide.thy
@@ -69,17 +69,17 @@ sepref_definition vmtf_find_next_undef_upd_code
         option_assn uint32_nat_assn\<close>
   supply [[goals_limit=1]]
   supply not_is_None_not_None[simp]
-  unfolding vmtf_find_next_undef_upd_def PR_CONST_def
+  unfolding isa_vmtf_find_next_undef_upd_def PR_CONST_def
   by sepref
 
 sepref_definition vmtf_find_next_undef_upd_fast_code
-  is \<open>uncurry (PR_CONST vmtf_find_next_undef_upd)\<close>
-  :: \<open>trail_fast_assn\<^sup>d *\<^sub>a vmtf_remove_conc\<^sup>d \<rightarrow>\<^sub>a
-     (trail_fast_assn *a vmtf_remove_conc) *a
+  is \<open>uncurry isa_vmtf_find_next_undef_upd\<close>
+  :: \<open>trail_pol_fast_assn\<^sup>d *\<^sub>a vmtf_remove_conc\<^sup>d \<rightarrow>\<^sub>a
+     (trail_pol_fast_assn *a vmtf_remove_conc) *a
         option_assn uint32_nat_assn\<close>
   supply [[goals_limit=1]]
   supply not_is_None_not_None[simp]
-  unfolding vmtf_find_next_undef_upd_def PR_CONST_def
+  unfolding isa_vmtf_find_next_undef_upd_def PR_CONST_def
   by sepref
 
 declare vmtf_find_next_undef_upd_code.refine[sepref_fr_rules]
@@ -90,19 +90,18 @@ definition lit_of_found_atm where
     (L \<noteq> None \<longrightarrow> K \<noteq> None \<and> atm_of (the K) = the L))\<close>
 
 definition find_undefined_atm
-  :: \<open>(nat,nat) ann_lits \<Rightarrow> vmtf_remove_int \<Rightarrow>
+  :: \<open>nat multiset \<Rightarrow> (nat,nat) ann_lits \<Rightarrow> vmtf_remove_int \<Rightarrow>
        (((nat,nat) ann_lits \<times> vmtf_remove_int) \<times> nat option) nres\<close>
 where
-  \<open>find_undefined_atm M _ = SPEC(\<lambda>((M', vm), L).
-     (L \<noteq> None \<longrightarrow> Pos (the L) \<in># \<L>\<^sub>a\<^sub>l\<^sub>l \<and> undefined_atm M (the L)) \<and>
-     (L = None \<longrightarrow> (\<forall>K\<in># \<L>\<^sub>a\<^sub>l\<^sub>l. defined_lit M K)) \<and> M = M' \<and> vm \<in> vmtf M)\<close>
+  \<open>find_undefined_atm \<A> M _ = SPEC(\<lambda>((M', vm), L).
+     (L \<noteq> None \<longrightarrow> Pos (the L) \<in># \<L>\<^sub>a\<^sub>l\<^sub>l \<A> \<and> undefined_atm M (the L)) \<and>
+     (L = None \<longrightarrow> (\<forall>K\<in># \<L>\<^sub>a\<^sub>l\<^sub>l \<A>. defined_lit M K)) \<and> M = M' \<and> vm \<in> vmtf \<A> M)\<close>
 
 definition find_unassigned_lit_wl_D_heur
   :: \<open>twl_st_wl_heur \<Rightarrow> (twl_st_wl_heur \<times> nat literal option) nres\<close>
 where
   \<open>find_unassigned_lit_wl_D_heur = (\<lambda>(M, N, D, WS, Q, vm, \<phi>, clvls). do {
-      ASSERT(vm \<in> vmtf M \<and> phase_saving \<phi>);
-      ((M, vm), L) \<leftarrow> find_undefined_atm M vm;
+      ((M, vm), L) \<leftarrow> isa_vmtf_find_next_undef_upd M vm;
       L \<leftarrow> lit_of_found_atm \<phi> L;
       RETURN ((M, N, D, WS, Q, vm, \<phi>, clvls), L)
     })\<close>
@@ -114,15 +113,64 @@ definition find_unassigned_lit_wl_D_heur_pre where
         (S, T) \<in> state_wl_l None \<and>
         (T, U) \<in> twl_st_l None \<and>
         twl_struct_invs U \<and>
-        literals_are_\<L>\<^sub>i\<^sub>n S \<and>
+        literals_are_\<L>\<^sub>i\<^sub>n (all_atms_st S) S \<and>
         get_conflict_wl S = None
     )\<close>
+
+lemma vmtf_find_next_undef_upd:
+  \<open>(uncurry (vmtf_find_next_undef_upd \<A>), uncurry (find_undefined_atm \<A>)) \<in>
+     [\<lambda>(M, vm). vm \<in> vmtf \<A> M]\<^sub>f Id \<times>\<^sub>f Id \<rightarrow> \<langle>Id \<times>\<^sub>f Id \<times>\<^sub>f \<langle>nat_rel\<rangle>option_rel\<rangle>nres_rel\<close>
+  unfolding vmtf_find_next_undef_upd_def find_undefined_atm_def
+    update_next_search_def uncurry_def
+  apply (intro frefI nres_relI)
+  apply (clarify)
+  apply (rule bind_refine_spec)
+   prefer 2
+   apply (rule vmtf_find_next_undef_ref[simplified])
+  by (auto intro!: RETURN_SPEC_refine simp: image_image defined_atm_def[symmetric])
+
+(*TODO Move*)
+lemma atm_of_all_lits_of_mm:
+  \<open>set_mset (atm_of `# all_lits_of_mm bw) = atms_of_mm bw\<close>
+  \<open>atm_of ` set_mset (all_lits_of_mm bw) = atms_of_mm bw\<close>
+  using in_all_lits_of_mm_ain_atms_of_iff apply (auto simp: image_iff)
+  by (metis (full_types) image_eqI literal.sel(1))+
+
+lemma \<L>\<^sub>a\<^sub>l\<^sub>l_union:
+   \<open>set_mset (\<L>\<^sub>a\<^sub>l\<^sub>l (A + B)) = set_mset (\<L>\<^sub>a\<^sub>l\<^sub>l  A) \<union> set_mset (\<L>\<^sub>a\<^sub>l\<^sub>l  B)\<close>
+  by (auto simp: \<L>\<^sub>a\<^sub>l\<^sub>l_def)
+
+lemma \<L>\<^sub>a\<^sub>l\<^sub>l_cong:
+  \<open>set_mset A = set_mset B \<Longrightarrow> set_mset (\<L>\<^sub>a\<^sub>l\<^sub>l A) = set_mset (\<L>\<^sub>a\<^sub>l\<^sub>l B)\<close>
+  by (auto simp: \<L>\<^sub>a\<^sub>l\<^sub>l_def)
+
+lemma lit_eq_Neg_Pos_iff:
+  \<open>x \<noteq> Neg (atm_of x) \<longleftrightarrow> is_pos x\<close>
+  \<open>x \<noteq> Pos (atm_of x) \<longleftrightarrow> is_neg x\<close>
+  \<open>-x \<noteq> Neg (atm_of x) \<longleftrightarrow> is_neg x\<close>
+  \<open>-x \<noteq> Pos (atm_of x) \<longleftrightarrow> is_pos x\<close>
+  \<open>Neg (atm_of x) \<noteq> x \<longleftrightarrow> is_pos x\<close>
+  \<open>Pos (atm_of x) \<noteq> x \<longleftrightarrow> is_neg x\<close>
+  \<open>Neg (atm_of x) \<noteq> -x \<longleftrightarrow> is_neg x\<close>
+  \<open>Pos (atm_of x) \<noteq> -x \<longleftrightarrow> is_pos x\<close>
+  by (cases x; auto; fail)+
+
+lemma \<L>\<^sub>a\<^sub>l\<^sub>l_atm_of_all_lits_of_m:
+   \<open>set_mset (\<L>\<^sub>a\<^sub>l\<^sub>l (atm_of `# all_lits_of_m C)) = set_mset C \<union> uminus ` set_mset C\<close>
+  supply lit_eq_Neg_Pos_iff[iff]
+  by (auto simp: \<L>\<^sub>a\<^sub>l\<^sub>l_def all_lits_of_m_def image_iff dest!: multi_member_split)
+
+lemma in_set_all_atms_iff:
+  \<open>y \<in># all_atms bu bw \<longleftrightarrow>
+    y \<in> atms_of_mm (mset `# ran_mf bu) \<or> y \<in> atms_of_mm bw\<close>
+  by (auto simp: all_atms_def all_lits_def in_all_lits_of_mm_ain_atms_of_iff
+     atm_of_all_lits_of_mm)
 
 lemma find_unassigned_lit_wl_D'_find_unassigned_lit_wl_D:
   \<open>(find_unassigned_lit_wl_D_heur, find_unassigned_lit_wl_D) \<in>
      [find_unassigned_lit_wl_D_heur_pre]\<^sub>f
     twl_st_heur''' r \<rightarrow> \<langle>{((T, L), (T', L')). (T, T') \<in> twl_st_heur''' r  \<and> L = L' \<and>
-         (L \<noteq> None \<longrightarrow> undefined_lit (get_trail_wl T') (the L) \<and> the L \<in># \<L>\<^sub>a\<^sub>l\<^sub>l) \<and>
+         (L \<noteq> None \<longrightarrow> undefined_lit (get_trail_wl T') (the L) \<and> the L \<in># \<L>\<^sub>a\<^sub>l\<^sub>l (all_atms_st T')) \<and>
          get_conflict_wl T' = None}\<rangle>nres_rel\<close>
 proof -
   have [simp]: \<open>undefined_lit M (Pos (atm_of y)) = undefined_lit M y\<close> for M y
@@ -132,17 +180,21 @@ proof -
 
   have ID_R: \<open>Id \<times>\<^sub>r \<langle>Id\<rangle>option_rel = Id\<close>
     by auto
-  have atms: \<open>atms_of \<L>\<^sub>a\<^sub>l\<^sub>l =
+  have atms: \<open>atms_of (\<L>\<^sub>a\<^sub>l\<^sub>l (all_atms_st (M, N, D, NE, UE, WS, Q))) =
          atms_of_mm (mset `# init_clss_lf N) \<union>
-         atms_of_mm NE \<and> D = None\<close>
+         atms_of_mm NE \<and> D = None\<close> (is ?A) and
+    atms_2: \<open>set_mset (\<L>\<^sub>a\<^sub>l\<^sub>l (all_atms N (NE + UE))) = set_mset (\<L>\<^sub>a\<^sub>l\<^sub>l (all_atms N NE))\<close> (is ?B) and
+    atms_3: \<open>y \<in> atms_of_ms ((\<lambda>x. mset (fst x)) ` set_mset (ran_m N)) \<Longrightarrow>
+       y \<notin> atms_of_mm NE \<Longrightarrow>
+       y \<in> atms_of_ms ((\<lambda>x. mset (fst x)) ` {a. a \<in># ran_m N \<and> snd a})\<close> (is \<open>?C1 \<Longrightarrow> ?C2 \<Longrightarrow>	?C\<close>)
       if inv: \<open>find_unassigned_lit_wl_D_heur_pre (M, N, D, NE, UE, WS, Q)\<close>
-      for M N D NE UE WS Q
+      for M N D NE UE WS Q y
   proof -
     obtain T U where
       S_T: \<open>((M, N, D, NE, UE, WS, Q), T) \<in> state_wl_l None\<close> and
       T_U: \<open>(T, U) \<in> twl_st_l None\<close> and
       inv: \<open>twl_struct_invs U\<close> and
-      \<A>\<^sub>i\<^sub>n : \<open>literals_are_\<L>\<^sub>i\<^sub>n (M, N, D, NE, UE, WS, Q)\<close> and
+      \<A>\<^sub>i\<^sub>n : \<open>literals_are_\<L>\<^sub>i\<^sub>n (all_atms_st (M, N, D, NE, UE, WS, Q)) (M, N, D, NE, UE, WS, Q)\<close> and
       confl: \<open>get_conflict_wl (M, N, D, NE, UE, WS, Q) = None\<close>
       using inv unfolding find_unassigned_lit_wl_D_heur_pre_def
        apply - apply normalize_goal+
@@ -152,43 +204,176 @@ proof -
         unit: \<open>entailed_clss_inv U\<close>
       using inv unfolding twl_struct_invs_def cdcl\<^sub>W_restart_mset.cdcl\<^sub>W_all_struct_inv_def
       by fast+
-    then show ?thesis
+    then show ?A
       using \<A>\<^sub>i\<^sub>n confl S_T T_U unfolding is_\<L>\<^sub>a\<^sub>l\<^sub>l_alt_def state_wl_l_def twl_st_l_def
-      literals_are_\<L>\<^sub>i\<^sub>n_def
+      literals_are_\<L>\<^sub>i\<^sub>n_def all_atms_def all_lits_def
       apply -
-      by (subst (asm) all_clss_l_ran_m[symmetric], subst (asm) image_mset_union)
-        (auto simp: cdcl\<^sub>W_restart_mset.no_strange_atm_def entailed_clss_inv.simps
-          mset_take_mset_drop_mset mset_take_mset_drop_mset'
+      apply (subst (asm) all_clss_l_ran_m[symmetric], subst (asm) image_mset_union)+
+      apply (subst all_clss_l_ran_m[symmetric], subst image_mset_union)
+      by  (auto simp: cdcl\<^sub>W_restart_mset.no_strange_atm_def entailed_clss_inv.simps
+          mset_take_mset_drop_mset mset_take_mset_drop_mset' atms_of_\<L>\<^sub>a\<^sub>l\<^sub>l_\<A>\<^sub>i\<^sub>n
           clauses_def simp del: entailed_clss_inv.simps)
+    then show ?B and \<open>?C1 \<Longrightarrow> ?C2 \<Longrightarrow> ?C\<close>
+      apply -
+      unfolding atms_of_\<L>\<^sub>a\<^sub>l\<^sub>l_\<A>\<^sub>i\<^sub>n all_atms_def all_lits_def
+      apply (subst (asm) all_clss_l_ran_m[symmetric], subst (asm) image_mset_union)+
+      apply (subst all_clss_l_ran_m[symmetric], subst image_mset_union)+
+      by (auto simp: in_\<L>\<^sub>a\<^sub>l\<^sub>l_atm_of_\<A>\<^sub>i\<^sub>n all_atms_def all_lits_def in_all_lits_of_mm_ain_atms_of_iff
+        all_lits_of_mm_union atms_of_def \<L>\<^sub>a\<^sub>l\<^sub>l_union image_Un atm_of_eq_atm_of
+	atm_of_all_lits_of_mm atms_of_\<L>\<^sub>a\<^sub>l\<^sub>l_\<A>\<^sub>i\<^sub>n)
   qed
 
-  have [dest]: \<open>(S, T) \<in> twl_st_heur \<Longrightarrow> \<phi> = get_phase_saver_heur S \<Longrightarrow> phase_saving \<phi>\<close> for S T \<phi>
-    by (auto simp: twl_st_heur_def)
+  have [dest]: \<open>(S, T) \<in> twl_st_heur \<Longrightarrow> \<phi> = get_phase_saver_heur S \<Longrightarrow> phase_saving (all_atms_st T) \<phi>\<close> for S T \<phi>
+    by (auto simp: twl_st_heur_def all_atms_def)
+  define unassigned_atm where
+    \<open>unassigned_atm S L \<equiv> \<exists> M N D NE UE WS Q.
+         S = (M, N, D, NE, UE, WS, Q) \<and>
+         (L \<noteq> None \<longrightarrow>
+            undefined_lit M (the L) \<and> the L \<in># \<L>\<^sub>a\<^sub>l\<^sub>l (all_atms N NE) \<and>
+            atm_of (the L) \<in> atms_of_mm (clause `# twl_clause_of `# init_clss_lf N + NE)) \<and>
+         (L = None \<longrightarrow> (\<nexists>L'. undefined_lit M L' \<and>
+            atm_of L' \<in> atms_of_mm (clause `# twl_clause_of `# init_clss_lf N + NE)))\<close>
+    for L :: \<open>nat literal option\<close> and S :: \<open>nat twl_st_wl\<close>
+  have find_unassigned_lit_wl_D_alt_def:
+   \<open>find_unassigned_lit_wl_D S = do {
+     L \<leftarrow>  SPEC(unassigned_atm S);
+     L \<leftarrow> RES {L, map_option uminus L};
+     SPEC(\<lambda>((M, N, D, NE, UE, WS, Q), L').
+         S = (M, N, D, NE, UE, WS, Q) \<and> L = L')
+   }\<close> for S
+   unfolding find_unassigned_lit_wl_D_def RES_RES_RETURN_RES unassigned_atm_def
+    RES_RES_RETURN_RES
+    by (cases S) (auto simp: mset_take_mset_drop_mset' uminus_\<A>\<^sub>i\<^sub>n_iff) 
 
+  have isa_vmtf_find_next_undef_upd:
+    \<open>isa_vmtf_find_next_undef_upd (a, aa, ab, ac, ad, b)
+       ((aj, ak, al, am, bb), an, bc)
+      \<le> \<Down> {(((M, vm), A), L). A = map_option atm_of L \<and>
+              unassigned_atm (bt, bu, bv, bw, bx, by, bz) L \<and>
+             vm \<in> isa_vmtf (all_atms_st (bt, bu, bv, bw, bx, by, bz)) bt \<and>
+             (M, bt) \<in> trail_pol (all_atms_st (bt, bu, bv, bw, bx, by, bz))}
+         (SPEC (unassigned_atm (bt, bu, bv, bw, bx, by, bz)))\<close>
+    if 
+      pre: \<open>find_unassigned_lit_wl_D_heur_pre (bt, bu, bv, bw, bx, by, bz)\<close> and
+      T: \<open>(((a, aa, ab, ac, ad, b), ae, (af, ag, ba), ah, ai,
+	 ((aj, ak, al, am, bb), an, bc), ao, ap, (aq, bd), ar, as,
+	 (at, au, av, aw, be), (ax, ay, az, bf, bg), (bh, bi, bj, bk, bl),
+	 (bm, bn), bo, bp, bq, br, bs),
+	bt, bu, bv, bw, bx, by, bz)
+       \<in> twl_st_heur\<close> and
+      \<open>r =
+       length
+	(get_clauses_wl_heur
+	  ((a, aa, ab, ac, ad, b), ae, (af, ag, ba), ah, ai,
+	   ((aj, ak, al, am, bb), an, bc), ao, ap, (aq, bd), ar, as,
+	   (at, au, av, aw, be), (ax, ay, az, bf, bg), (bh, bi, bj, bk, bl),
+	   (bm, bn), bo, bp, bq, br, bs))\<close>
+     for a aa ab ac ad b ae af ag ba ah ai aj ak al am bb an bc ao ap aq bd ar as at
+	 au av aw be ax ay az bf bg bh bi bj bk bl bm bn bo bp bq br bs bt bu bv
+	 bw bx "by" bz
+  proof -
+    let ?\<A> = \<open>all_atms_st (bt, bu, bv, bw, bx, by, bz)\<close>
+    have pol:
+      \<open>((a, aa, ab, ac, ad, b), bt) \<in> trail_pol (all_atms bu (bw + bx))\<close>
+      using that by (auto simp: twl_st_heur_def all_atms_def[symmetric])
+    obtain vm0 where
+      vm0: \<open>((an, bc), vm0) \<in> distinct_atoms_rel (all_atms bu (bw + bx))\<close> and
+      vm: \<open>((aj, ak, al, am, bb), vm0) \<in> vmtf (all_atms bu (bw + bx)) bt\<close>
+      using T by (auto simp: twl_st_heur_def all_atms_def[symmetric] isa_vmtf_def)
+    have [intro]: \<open>Multiset.Ball (\<L>\<^sub>a\<^sub>l\<^sub>l (all_atms bu (bw + bx))) (defined_lit bt) \<Longrightarrow>
+	 atm_of L'
+	 \<in> atms_of_ms ((\<lambda>x. mset (fst x)) ` {a. a \<in># ran_m bu \<and> snd a}) \<Longrightarrow>
+		undefined_lit bt L' \<Longrightarrow> False\<close>
+       \<open>Multiset.Ball (\<L>\<^sub>a\<^sub>l\<^sub>l (all_atms bu (bw + bx))) (defined_lit bt) \<Longrightarrow>
+	 atm_of L'
+	 \<in> atms_of_mm bw \<Longrightarrow>
+		undefined_lit bt L' \<Longrightarrow> False\<close>
+       \<open>Multiset.Ball (\<L>\<^sub>a\<^sub>l\<^sub>l (all_atms bu (bw + bx))) (defined_lit bt) \<Longrightarrow>
+	 atm_of L'
+	 \<in> atms_of_mm bx \<Longrightarrow>
+		undefined_lit bt L'\<Longrightarrow> False\<close> for L'
+      by (auto simp: all_atms_def atms_of_ms_def atm_of_eq_atm_of all_lits_def
+	   all_lits_of_mm_union ran_m_def all_lits_of_mm_add_mset \<L>\<^sub>a\<^sub>l\<^sub>l_union
+	   eq_commute[of _ \<open>the (fmlookup _ _)\<close>] \<L>\<^sub>a\<^sub>l\<^sub>l_atm_of_all_lits_of_m
+	  atms_of_def
+	 dest!: multi_member_split
+	  )
+
+    show ?thesis
+      apply (rule order.trans)
+      apply (rule isa_vmtf_find_next_undef_vmtf_find_next_undef[of ?\<A>, THEN fref_to_Down_curry,
+	 of _ _ bt \<open>((aj, ak, al, am, bb), vm0)\<close>])
+      subgoal by fast
+      subgoal
+	 using pol vm0 by (auto simp: twl_st_heur_def all_atms_def[symmetric])
+      apply (rule order.trans)
+      apply (rule ref_two_step')
+      apply (rule vmtf_find_next_undef_upd[THEN fref_to_Down_curry, of ?\<A> bt \<open>((aj, ak, al, am, bb), vm0)\<close>])
+      subgoal using vm by (auto simp: all_atms_def)
+      subgoal by auto
+      subgoal using vm vm0 pre
+	apply (auto 5 0 simp: find_undefined_atm_def unassigned_atm_def conc_fun_RES all_atms_def[symmetric]
+	   mset_take_mset_drop_mset' atms_2 defined_atm_def
+	   intro!: RES_refine intro: isa_vmtfI)
+	apply (auto intro: isa_vmtfI simp: defined_atm_def atms_2)
+	apply (rule_tac x = \<open>Some (Pos y)\<close> in exI)
+	apply (auto intro: isa_vmtfI simp: defined_atm_def atms_2  in_\<L>\<^sub>a\<^sub>l\<^sub>l_atm_of_\<A>\<^sub>i\<^sub>n
+	 in_set_all_atms_iff atms_3)
+	done
+    done
+  qed
+
+  have lit_of_found_atm: \<open>lit_of_found_atm ao x2a
+	\<le> \<Down> {(L, L'). L = L' \<and> map_option atm_of  L = x2a}
+	   (RES {L, map_option uminus L})\<close>
+    if 
+      \<open>find_unassigned_lit_wl_D_heur_pre (bt, bu, bv, bw, bx, by, bz)\<close> and
+      \<open>(((a, aa, ab, ac, ad, b), ae, (af, ag, ba), ah, ai,
+	 ((aj, ak, al, am, bb), an, bc), ao, ap, (aq, bd), ar, as,
+	 (at, au, av, aw, be), (ax, ay, az, bf, bg), (bh, bi, bj, bk, bl),
+	 (bm, bn), bo, bp, bq, br, bs),
+	bt, bu, bv, bw, bx, by, bz)
+       \<in> twl_st_heur\<close> and
+      \<open>r =
+       length
+	(get_clauses_wl_heur
+	  ((a, aa, ab, ac, ad, b), ae, (af, ag, ba), ah, ai,
+	   ((aj, ak, al, am, bb), an, bc), ao, ap, (aq, bd), ar, as,
+	   (at, au, av, aw, be), (ax, ay, az, bf, bg), (bh, bi, bj, bk, bl),
+	   (bm, bn), bo, bp, bq, br, bs))\<close> and
+      \<open>(x, L)
+       \<in> {(((M, vm), A), L).
+	  A = map_option atm_of L \<and>
+	  unassigned_atm (bt, bu, bv, bw, bx, by, bz) L \<and>
+	  vm \<in> isa_vmtf (all_atms_st (bt, bu, bv, bw, bx, by, bz)) bt \<and>
+	  (M, bt) \<in> trail_pol (all_atms_st (bt, bu, bv, bw, bx, by, bz))}\<close> and
+      \<open>L \<in> Collect (unassigned_atm (bt, bu, bv, bw, bx, by, bz))\<close> and
+      \<open>x1 = (x1a, x2)\<close> and
+      \<open>x = (x1, x2a)\<close>
+     for a aa ab ac ad b ae af ag ba ah ai aj ak al am bb an bc ao ap aq bd ar as at
+       au av aw be ax ay az bf bg bh bi bj bk bl bm bn bo bp bq br bs bt bu bv
+       bw bx "by" bz x L x1 x1a x2 x2a
+  proof -
+    show ?thesis
+      using that unfolding lit_of_found_atm_def
+      by (auto simp: atm_of_eq_atm_of twl_st_heur_def intro!: RES_refine)
+  qed
   show ?thesis
-    unfolding find_unassigned_lit_wl_D_heur_def find_unassigned_lit_wl_D_def find_undefined_atm_def
-      ID_R lit_of_found_atm_def
+    unfolding find_unassigned_lit_wl_D_heur_def find_unassigned_lit_wl_D_alt_def find_undefined_atm_def
+      ID_R
     apply (intro frefI nres_relI)
     apply clarify
     apply refine_vcg
-    unfolding RETURN_RES_refine_iff
-    by (auto simp add: twl_st_heur_def in_\<L>\<^sub>a\<^sub>l\<^sub>l_atm_of_in_atms_of_iff Ball_def image_image
-        mset_take_mset_drop_mset' atms
-          simp del: twl_st_of_wl.simps dest!: atms)
+    apply (rule isa_vmtf_find_next_undef_upd; assumption)
+    apply (rule lit_of_found_atm; assumption)
+    subgoal
+      by (auto simp add: twl_st_heur_def in_\<L>\<^sub>a\<^sub>l\<^sub>l_atm_of_in_atms_of_iff Ball_def image_image
+        mset_take_mset_drop_mset' atms all_atms_def[symmetric] unassigned_atm_def
+        atm_of_eq_atm_of
+          simp del: twl_st_of_wl.simps dest!: atms intro!: RETURN_RES_refine)
+    done
 qed
 
-
-lemma vmtf_find_next_undef_upd:
-  \<open>(uncurry vmtf_find_next_undef_upd, uncurry find_undefined_atm) \<in>
-     [\<lambda>(M, vm). vm \<in> vmtf M]\<^sub>f Id \<times>\<^sub>f Id \<rightarrow> \<langle>Id \<times>\<^sub>f Id \<times>\<^sub>f \<langle>nat_rel\<rangle>option_rel\<rangle>nres_rel\<close>
-  unfolding vmtf_find_next_undef_upd_def trail_ref_except_ann_lits_def find_undefined_atm_def
-    update_next_search_def uncurry_def
-  apply (intro frefI nres_relI)
-  apply (clarify)
-  apply (rule bind_refine_spec)
-   prefer 2
-   apply (rule vmtf_find_next_undef_ref[simplified])
-  by (auto intro!: RETURN_SPEC_refine simp: image_image defined_atm_def[symmetric])
 
 
 lemma find_undefined_atm_hnr[sepref_fr_rules]:
